WIP

src/Specific/GF25519Reflective/Reified/rebuild-reified.py
@@ -9,22 +9,27 @@ for name, opkind in ([(name, 'BinOp') for name in ('Add', 'Carry_Add', 'Sub', 'C
     uopkind = opkind.replace('_', '')
     extra = ''
     #if name in ('Carry_Add', 'Carry_Sub', 'Mul', 'Carry_Opp', 'Pack', 'Unpack', 'Ge_Modulus', 'PreFreeze'):
-    extra = r"""Local Obligation Tactic := intros; vm_compute; constructor.
-Program Definition r%(lname)sZ_correct_and_bounded
-  := rexpr_correct_and_bounded r%(lname)sZ r%(lname)sZ_Wf Expr%(uopkind)s_bounds.
+    extra = r"""Local Obligation Tactic := rexpr_correct_and_bounded_obligation_tac.
+Program Definition r%(lname)sZ_correct_and_bounded_tight
+  : rexpr_correct_and_boundedT r%(lname)sZ r%(lname)sW Expr%(uopkind)s_bounds r%(lname)s_output_bounds
+  := rexpr_correct_and_bounded r%(lname)sZ r%(lname)sW Expr%(uopkind)s_bounds r%(lname)s_output_bounds r%(lname)sZ_Wf.
 """ % locals()
     with open(name.replace('_', '') + '.v', 'w') as f:
         f.write(r"""Require Import Crypto.Specific.GF25519Reflective.Common.
 
 Definition r%(lname)sZ_sig : rexpr_%(lopkind)s_sig %(lname)s. Proof. reify_sig. Defined.
-Definition r%(lname)sZ : Syntax.Expr _ _ _ := Eval vm_compute in proj1_sig r%(lname)sZ_sig.
-Definition r%(lname)sW : Syntax.Expr _ _ _ := Eval vm_compute in rexpr_select_word_sizes r%(lname)sZ Expr%(uopkind)s_bounds.
+Definition r%(lname)sZ : Expr _ := Eval vm_compute in proj1_sig r%(lname)sZ_sig.
+Definition r%(lname)sW_pkgo := Eval vm_compute in rexpr_select_word_sizes_option r%(lname)sZ Expr%(uopkind)s_bounds.
+Definition r%(lname)sW_pkg := Eval vm_compute in rexpr_select_word_sizes_postprocess1 r%(lname)sW_pkgo.
+Definition r%(lname)sT := get_output_type r%(lname)sW_pkg.
+Definition r%(lname)sW' : Expr _ := Eval vm_compute in get_output_expr r%(lname)sW_pkg.
+Definition r%(lname)sW : Expr r%(lname)sT := Eval cbv [r%(lname)sW'] in rexpr_select_word_sizes_postprocess2 r%(lname)sW'.
+Definition r%(lname)s_output_bounds := Eval vm_compute in get_bounds r%(lname)sW_pkg.
 Definition r%(lname)sZ_Wf : rexpr_wfT r%(lname)sZ. Proof. prove_rexpr_wfT. Qed.
-Definition r%(lname)s_output_bounds
-  := Eval vm_compute in compute_bounds r%(lname)sZ Expr%(uopkind)s_bounds.
 %(extra)s
 Local Open Scope string_scope.
-Compute ("%(name)s", compute_bounds_for_display r%(lname)sZ Expr%(uopkind)s_bounds).
-Compute ("%(name)s overflows? ", sanity_compute r%(lname)sZ Expr%(uopkind)s_bounds).
-Compute ("%(name)s overflows (error if it does)? ", sanity_check r%(lname)sZ Expr%(uopkind)s_bounds).
+Compute ("%(name)s", compute_bounds_for_display r%(lname)sW_pkg).
+(* We use [compute] rather than [vm_compute] so as to not eta-expand functions, so we get pretty display *)
+Eval compute in ("%(name)s overflows? ", sanity_compute r%(lname)sW_pkg).
+Compute ("%(name)s overflows (error if it does)? ", sanity_check r%(lname)sW_pkg).
 """ % locals())
