src/Specific/IntegrationTest.v
@@ -13,8 +13,8 @@ Import ListNotations.
 Section Pre.
   Definition BoundedWord n (bitwidth : nat)
              (bounds : tuple zrange n) : Type :=
-    { x : tuple (wordT bitwidth) n
-    | is_bounded_by (Some (Z.of_nat bitwidth)) bounds
+    { x : tuple (wordT (Nat.log2 bitwidth)) n
+    | is_bounded_by None bounds
                     (map wordToZ x)}.
 
   Definition BoundedWordToZ n w b (BW :BoundedWord n w b)
@@ -46,17 +46,298 @@ Section BoundedField25p5.
     fun x => B.Positional.Fdecode wt (BoundedWordToZ _ _ _ x).
 
   (* TODO : change this to field once field isomorphism happens *)
-  Definition mul :
-    { mul : feBW -> feBW -> feBW
-    | forall a b, phi (mul a b) = (phi a * phi b)%F }.
+  Definition add :
+    { add : feBW -> feBW -> feBW
+    | forall a b, phi (add a b) = (phi a + phi b)%F }.
   Proof.
-    eexists ?[mul]; intros. cbv [phi].
-    rewrite <- (proj2_sig mul_sig).
-    set (mulZ := proj1_sig mul_sig).
-    cbv beta iota delta [proj1_sig mul_sig runtime_add runtime_and runtime_mul runtime_opp runtime_shr] in mulZ.
+    eexists ?[add]; intros. cbv [phi].
+    rewrite <- (proj2_sig add_sig).
+    symmetry; rewrite <- (proj2_sig carry_sig); symmetry.
+    set (carry_addZ := fun a b => proj1_sig carry_sig (proj1_sig add_sig a b)).
+    change (proj1_sig carry_sig (proj1_sig add_sig ?a ?b)) with (carry_addZ a b).
+    (* XXX FIXME This is a kludge around anomalies in Coq *)
+    Definition recurry1 {T} (F : Z * Z * Z * Z * Z * Z * Z * Z * Z * Z -> T) (x : Z * Z * Z * Z * Z * Z * Z * Z * Z * Z) : T
+      := let '(a, b, c, d, e, f, g, h, i, j) := x in
+         F ((a, b, c, d, e, f, g, h, i, j)).
+    Definition recurry {T} (F : Z * Z * Z * Z * Z * Z * Z * Z * Z * Z * (Z * Z * Z * Z * Z * Z * Z * Z * Z * Z) -> T) (x : Z * Z * Z * Z * Z * Z * Z * Z * Z * Z * (Z * Z * Z * Z * Z * Z * Z * Z * Z * Z)) : T
+      := let '(a, b, c, d, e, f, g, h, i, j) := fst x in
+         let '(a', b', c', d', e', f', g', h', i', j') := snd x in
+         F ((a, b, c, d, e, f, g, h, i, j, (a', b', c', d', e', f', g', h', i', j'))).
+    change (proj1_sig carry_sig) with (recurry1 (proj1_sig carry_sig)) in (value of carry_addZ).
+    change (proj1_sig add_sig) with (fun x y => recurry (fun xy => proj1_sig add_sig (fst xy) (snd xy)) (x, y)) in (value of carry_addZ).
+    cbv beta iota delta [proj1_sig add_sig carry_sig recurry recurry1 runtime_add runtime_and runtime_mul runtime_opp runtime_shr sz] in carry_addZ.
+    cbn beta iota delta [fst snd] in carry_addZ.
     apply f_equal.
     (* jgross start here! *)
+    Require Import Crypto.Util.LetIn.
+    Require Import Crypto.Reflection.Z.Syntax.Util.
+    Require Import Crypto.Util.Tactics.Head.
+    Require Import Crypto.Util.Curry.
+    Require Import Crypto.Util.Tactics.ETransitivity.
+    Require Import Crypto.Reflection.Syntax.
+    Require Import Crypto.Reflection.Z.Syntax.
+    Require Import Crypto.Reflection.Reify.
+    Require Import Crypto.Reflection.Z.Bounds.Interpretation.
+    Require Import Crypto.Reflection.Z.Reify.
 
+(** The [do_curry] tactic takes a goal of the form
+<<
+BoundedWordToZ (?f a b ... z) = F A B ... Z
+>>
+    and turns it into a goal of the form
+<<
+BoundedWordToZ (f' (a, b, ..., z)) = F' (A, B, ..., Z)
+>>
+ *)
+Ltac do_curry :=
+  lazymatch goal with
+  | [ |- ?BWtoZ ?f_bw = ?f_Z ]
+    => let f_bw := head f_bw in
+       let f_Z := head f_Z in
+       change_with_curried f_Z;
+       let f_bw_name := fresh f_bw in
+       set (f_bw_name := f_bw);
+       change_with_curried f_bw_name
+  end.
+(** The [split_BoundedWordToZ] tactic takes a goal of the form
+<<
+BoundedWordToZ (f args) = F ARGS
+>>
+    and splits it into a conjunction, one part about the computational
+    behavior, and another part about the boundedness.  *)
+Ltac count_tuple_length T :=
+  lazymatch T with
+  | (?A * ?B)%type => let a := count_tuple_length A in
+                      let b := count_tuple_length B in
+                      (eval compute in (a + b)%nat)
+  | _ => constr:(1%nat)
+  end.
+Ltac make_evar_for_first_projection :=
+  lazymatch goal with
+  | [ |- @map ?N1 ?A ?B wordToZ (@proj1_sig _ ?P (?f ?args)) = _ ]
+    => let T := type of args in
+       let N := count_tuple_length T in
+       let map' := (eval compute in (@map N)) in
+       let proj1_sig' := (eval compute in @proj1_sig) in
+       let pf := fresh in
+       let y := fresh in
+       refine (let y := @map N1 A B wordToZ (_ (map' _ _ (proj1_sig' _ _) args)) in _);
+       simple refine (let pf := _ in _);
+       [ shelve
+       | subst y f
+       | etransitivity_rev y;
+         subst y;
+         clearbody pf;
+         cbv beta iota;
+         [ lazymatch goal with
+           | [ |- ?map ?wordToZ (?f ?args) = ?RHS ]
+             => cut (P (f args) /\ map wordToZ (f args) = RHS); [ refine (@proj2 _ _) | exact pf ]
+           end
+         | subst f; cbn [fst snd]; apply f_equal;
+           instantiate (2:=ltac:(repeat intros [? ?]; refine (exist _ _ _)))(* XXX FIXME: Is 2 always the right number? *) ] ];
+       cbn [proj1_sig]
+  end.
+Ltac split_BoundedWordToZ :=
+  repeat match goal with
+         | [ |- context[BoundedWordToZ _ _ _ ?x] ]
+           => is_var x; destruct x
+         end;
+  unfold BoundedWordToZ; cbn [proj1_sig];
+  make_evar_for_first_projection.
+(** The [zrange_to_reflective] tactic takes a goal of the form
+<<
+is_bounded_by _ bounds (map wordToZ (?fW args)) /\ map wordToZ (?fW args) = fZ argsZ
+>>
+    and uses [change] to turn it into a goal that the reflective
+    machinery can handle.  The goal left by this tactic should be
+    fully solvable by the reflective pipeline. *)
+Ltac const_tuple T val :=
+  lazymatch T with
+  | (?A * ?B)%type => let a := const_tuple A val in
+                      let b := const_tuple B val in
+                      constr:((a, b)%core)
+  | _ => val
+  end.
+Lemma adjust_goal_for_reflective {T P} (LHS RHS : T)
+  : P RHS /\ LHS = RHS -> P LHS /\ LHS = RHS.
+Proof. intros [? ?]; subst; tauto. Qed.
+Ltac adjust_goal_for_reflective := apply adjust_goal_for_reflective.
+Ltac zrange_to_reflective :=
+  lazymatch goal with
+  | [ |- @ZRange.is_bounded_by ?option_bit_width ?count ?bounds (Tuple.map wordToZ (?reified_f_evar ?args))
+         /\ Tuple.map wordToZ (?reified_f_evar ?args) = ?f ?Zargs ]
+    => let T := type of f in
+       let f_domain := lazymatch T with ?A -> ?B => A end in
+       let T := (eval compute in T) in
+       let rT := reify_type T in
+       let is_bounded_by' := constr:(@Bounds.is_bounded_by (codomain rT)) in
+       let input_bounds := const_tuple f_domain bounds in
+       let map_t := constr:(fun t bs => @cast_back_flat_const (@Bounds.interp_base_type) t (fun _ => Bounds.bounds_to_base_type) bs) in
+       let map_output := constr:(map_t (codomain rT) bounds) in
+       let map_input := constr:(map_t (domain rT) input_bounds) in
+       change (is_bounded_by' bounds (map_output (reified_f_evar args)) /\ map_output (reified_f_evar args) = f (map_input args));
+       cbv beta
+  end;
+  adjust_goal_for_reflective.
+Require Import Crypto.Reflection.Z.Bounds.Relax.
+do_curry.
+split_BoundedWordToZ.
+zrange_to_reflective.
+
+Require Import Crypto.Reflection.Z.MapBounds.
+Require Import Crypto.Reflection.Z.MapBoundsInterp.
+Require Import Crypto.Reflection.RenameBinders.
+Require Import Crypto.Reflection.Wf.
+Require Import Crypto.Util.Option.
+Require Import Crypto.Reflection.WfReflective.
+Require Import Crypto.Reflection.SmartMap.
+
+Ltac rexpr_cbv :=
+  lazymatch goal with
+  | [ |- { rexpr | forall x, Interp _ (t:=?T) rexpr x = ?uncurry ?oper x } ]
+    => let operf := head oper in
+       let uncurryf := head uncurry in
+       try cbv delta [T]; try cbv delta [oper];
+       try cbv beta iota delta [uncurryf]
+  | [ |- { rexpr | forall x, Interp _ (t:=?T) rexpr x = ?oper x } ]
+    => let operf := head oper in
+       try cbv delta [T]; try cbv delta [oper]
+  end;
+  cbv beta iota delta [interp_flat_type interp_base_type].
+Ltac reify_sig :=
+  rexpr_cbv; eexists; Reify_rhs; reflexivity.
+Ltac assert_reflective :=
+  lazymatch goal with
+  | [ |- @Bounds.is_bounded_by (codomain ?T) ?bounds _
+         /\ cast_back_flat_const (?fW ?v) = ?fZ (cast_back_flat_const ?v) ]
+    => let rexpr := fresh "rexpr" in
+       simple refine (let rexpr : { rexpr | forall x, Interp interp_op (t:=T) rexpr x = fZ x } := _ in _);
+         [
+         | rewrite <- (proj2_sig rexpr);
+           let rexpr' := fresh rexpr in
+           set (rexpr' := proj1_sig rexpr);
+           unfold proj1_sig in rexpr';
+           subst rexpr fZ ]
+  end.
+Ltac prove_rexpr_wfT
+  := reflect_Wf Equality.base_type_eq_semidec_is_dec Equality.op_beq_bl.
+
+Ltac assert_wf :=
+  lazymatch goal with
+  | [ |- @Bounds.is_bounded_by (codomain ?T) ?bounds _
+         /\ cast_back_flat_const (?fW ?v) = Interp _ ?fZ (@cast_back_flat_const _ _ _ ?input_bounds ?v) ]
+    => assert (Wf fZ) by prove_rexpr_wfT
+  end.
+
+Notation rexpr_select_word_sizes_option rexprZ rexpr_bounds
+  := (Z.MapBounds.MapBoundsPackaged rexprZ rexpr_bounds)
+       (only parsing).
+Notation rexpr_select_word_sizes_postprocess1 v
+  := (invert_Some v)
+       (only parsing).
+Notation get_output_type v := (MapBoundsOutputType v) (only parsing).
+Notation get_bounds v := (@output_bounds v) (only parsing).
+Notation get_output_expr v := (@output_expr v) (only parsing).
+Notation rexpr_select_word_sizes_postprocess2 v
+  := (renamify v)
+       (only parsing).
+
+Local Notation pick_typeb := Bounds.bounds_to_base_type (only parsing).
+Local Notation pick_type v := (SmartFlatTypeMap (fun _ => pick_typeb) v).
+
+Notation rexpr_correct_and_boundedT rexprZ rexprW input_bounds output_bounds
+  := (let t := _ in
+      let e : Expr t := rexprZ in
+      let input_bounds : interp_flat_type Bounds.interp_base_type (domain t)
+          := input_bounds in
+      let output_bounds : interp_flat_type Bounds.interp_base_type (codomain t)
+          := output_bounds in
+      forall (v : interp_flat_type Syntax.interp_base_type (domain t))
+             (v' : interp_flat_type Syntax.interp_base_type (pick_type input_bounds)),
+         (Bounds.is_bounded_by input_bounds v /\ cast_back_flat_const v' = v)
+         -> Bounds.is_bounded_by output_bounds (Interp interp_op e v)
+            /\ cast_back_flat_const (Interp interp_op rexprW v') = Interp interp_op e v)
+       (only parsing).
+
+Notation rexpr_correct_and_bounded rexprZ rexprW input_bounds output_bounds rexprZ_Wf
+  := (fun v v' Hv
+      => proj2
+           (@MapBoundsPackagedCorrect
+              _ rexprZ input_bounds rexprZ_Wf
+              output_bounds rexprW
+              _
+              v v' Hv))
+       (only parsing).
+
+Ltac rexpr_correct_and_bounded_obligation_tac :=
+  intros;
+  lazymatch goal with
+  | [ |- ?x = Some ?y ]
+    => abstract vm_cast_no_check (eq_refl (Some y))
+  | _ => vm_compute; constructor
+  end.
+
+
+Ltac make_correctness rexprZ bounds Hcorrectness :=
+  let rexprW_pkgo := (eval vm_compute in (rexpr_select_word_sizes_option rexprZ bounds)) in
+  let rexprW_pkg := (eval vm_compute in (rexpr_select_word_sizes_postprocess1 rexprW_pkgo)) in
+  let rexprT := constr:(get_output_type rexprW_pkg) in
+  let rexprW' := (eval vm_compute in (get_output_expr rexprW_pkg)) in
+  let rexprW := (eval cbv beta iota zeta in (rexpr_select_word_sizes_postprocess2 rexprW')) in
+  let rexpr_output_bounds := (eval vm_compute in (get_bounds rexprW_pkg)) in
+  let rexprZ_Wf := lazymatch goal with H : Wf rexprZ |- _ => H end in
+  simple refine (let Hcorrectness := rexpr_correct_and_bounded rexprZ rexprW bounds rexpr_output_bounds rexprZ_Wf in _);
+  [ rexpr_correct_and_bounded_obligation_tac.. | clearbody Hcorrectness ].
+Ltac do_pose_correctness Hcorrectness :=
+  lazymatch goal with
+  | [ |- @Bounds.is_bounded_by (codomain ?T) ?bounds _
+         /\ cast_back_flat_const (?fW ?v) = Interp _ ?fZ (@cast_back_flat_const _ _ _ ?input_bounds ?v) ]
+    => make_correctness fZ input_bounds Hcorrectness
+  end.
+Ltac pretighten_bounds tighter_bounds :=
+  lazymatch goal with
+  | [ |- @Bounds.is_bounded_by ?t ?relaxed_bounds _ /\ cast_back_flat_const ?v = ?k ]
+    => simple refine (@relax_output_bounds t tighter_bounds relaxed_bounds _ v k _ _)
+  end.
+Ltac posttighten_bounds :=
+  [ > clear; vm_compute; reflexivity | unfold eq_rect | clear ].
+Ltac pretighten_bounds_from_correctness Hcorrectness :=
+  cbv beta iota zeta in Hcorrectness;
+  lazymatch type of Hcorrectness with
+  | forall v v', _ -> Bounds.is_bounded_by ?tighter_bounds _ /\ _
+    => pretighten_bounds tighter_bounds
+  end.
+Ltac tighten_bounds_from_correctness Hcorrectness :=
+  pretighten_bounds_from_correctness Hcorrectness; posttighten_bounds.
+Ltac specialize_Hcorrectness Hcorrectness :=
+  lazymatch goal with
+  | [ |- @Bounds.is_bounded_by (codomain ?T) ?bounds (Interp _ ?fZ ?v')
+         /\ cast_back_flat_const (?fW ?v) = Interp _ ?fZ ?v' ]
+    => specialize (Hcorrectness v' v);
+       lazymatch type of Hcorrectness with
+       | ?T -> Bounds.is_bounded_by _ _ /\ cast_back_flat_const (?fW' _) = _
+         => unify fW fW'; cut T
+       end;
+       [ let H := fresh in intro H; specialize (Hcorrectness H) | ]
+  end.
+assert_reflective.
+cbv [interp_flat_type interp_base_type Tuple.tuple Tuple.tuple'] in *.
+reify_sig.
+cbv beta iota in *.
+assert_wf.
+do_pose_correctness Hcorrectness.
+tighten_bounds_from_correctness Hcorrectness.
+specialize_Hcorrectness Hcorrectness.
+exact Hcorrectness.
+Ltac handle_bounds_from_hyps :=
+  repeat match goal with
+         | _ => assumption
+         | [ |- cast_back_flat_const _ = cast_back_flat_const _ ] => reflexivity
+         | [ |- _ /\ _ ] => split
+         | [ |- Bounds.is_bounded_by (_, _) _ ] => split
+         end.
+{ handle_bounds_from_hyps. }
+2:reflexivity.
   Admitted.
 
 End BoundedField25p5.
