src/Specific/GF25519Reflective/Reified/GeModulus.v
@@ -1,17 +1,21 @@
-Require Import Crypto.Specific.GF25519Reflective.CommonUnOpFEToZ.
+Require Import Crypto.Specific.GF25519Reflective.Common.
 
 Definition rge_modulusZ_sig : rexpr_unop_FEToZ_sig ge_modulus. Proof. reify_sig. Defined.
-Definition rge_modulusW := Eval vm_compute in rword_of_Z rge_modulusZ_sig.
-Lemma rge_modulusW_correct_and_bounded_gen : correct_and_bounded_genT rge_modulusW rge_modulusZ_sig.
-Proof. rexpr_correct. Qed.
-Definition rge_modulus_output_bounds := Eval vm_compute in compute_bounds rge_modulusW ExprUnOpFEToZ_bounds.
-Local Obligation Tactic := intros; vm_compute; constructor.
-Program Definition rge_modulusW_correct_and_bounded
-  := ExprUnOpFEToZ_correct_and_bounded
-       rge_modulusW ge_modulus rge_modulusZ_sig rge_modulusW_correct_and_bounded_gen
-       _ _.
+Definition rge_modulusZ : Expr _ := Eval vm_compute in proj1_sig rge_modulusZ_sig.
+Definition rge_modulusW_pkgo := Eval vm_compute in rexpr_select_word_sizes_option rge_modulusZ ExprUnOpFEToZ_bounds.
+Definition rge_modulusW_pkg := Eval vm_compute in rexpr_select_word_sizes_postprocess1 rge_modulusW_pkgo.
+Definition rge_modulusT := get_output_type rge_modulusW_pkg.
+Definition rge_modulusW' : Expr _ := Eval vm_compute in get_output_expr rge_modulusW_pkg.
+Definition rge_modulusW : Expr rge_modulusT := Eval cbv [rge_modulusW'] in rexpr_select_word_sizes_postprocess2 rge_modulusW'.
+Definition rge_modulus_output_bounds := Eval vm_compute in get_bounds rge_modulusW_pkg.
+Definition rge_modulusZ_Wf : rexpr_wfT rge_modulusZ. Proof. prove_rexpr_wfT. Qed.
+Local Obligation Tactic := rexpr_correct_and_bounded_obligation_tac.
+Program Definition rge_modulusZ_correct_and_bounded_tight
+  : rexpr_correct_and_boundedT rge_modulusZ rge_modulusW ExprUnOpFEToZ_bounds rge_modulus_output_bounds
+  := rexpr_correct_and_bounded rge_modulusZ rge_modulusW ExprUnOpFEToZ_bounds rge_modulus_output_bounds rge_modulusZ_Wf.
 
 Local Open Scope string_scope.
-Compute ("Ge_Modulus", compute_bounds_for_display rge_modulusW ExprUnOpFEToZ_bounds).
-Compute ("Ge_Modulus overflows? ", sanity_compute rge_modulusW ExprUnOpFEToZ_bounds).
-Compute ("Ge_Modulus overflows (error if it does)? ", sanity_check rge_modulusW ExprUnOpFEToZ_bounds).
+Compute ("Ge_Modulus", compute_bounds_for_display rge_modulusW_pkg).
+(* We use [compute] rather than [vm_compute] so as to not eta-expand functions, so we get pretty display *)
+Eval compute in ("Ge_Modulus overflows? ", sanity_compute rge_modulusW_pkg).
+Compute ("Ge_Modulus overflows (error if it does)? ", sanity_check rge_modulusW_pkg).
