src/Specific/GF25519Reflective/Reified/Opp.v
@@ -1,12 +1,21 @@
-Require Import Crypto.Specific.GF25519Reflective.CommonUnOp.
+Require Import Crypto.Specific.GF25519Reflective.Common.
 
 Definition roppZ_sig : rexpr_unop_sig opp. Proof. reify_sig. Defined.
-Definition roppW := Eval vm_compute in rword_of_Z roppZ_sig.
-Lemma roppW_correct_and_bounded_gen : correct_and_bounded_genT roppW roppZ_sig.
-Proof. rexpr_correct. Qed.
-Definition ropp_output_bounds := Eval vm_compute in compute_bounds roppW ExprUnOp_bounds.
+Definition roppZ : Expr _ := Eval vm_compute in proj1_sig roppZ_sig.
+Definition roppW_pkgo := Eval vm_compute in rexpr_select_word_sizes_option roppZ ExprUnOp_bounds.
+Definition roppW_pkg := Eval vm_compute in rexpr_select_word_sizes_postprocess1 roppW_pkgo.
+Definition roppT := get_output_type roppW_pkg.
+Definition roppW' : Expr _ := Eval vm_compute in get_output_expr roppW_pkg.
+Definition roppW : Expr roppT := Eval cbv [roppW'] in rexpr_select_word_sizes_postprocess2 roppW'.
+Definition ropp_output_bounds := Eval vm_compute in get_bounds roppW_pkg.
+Definition roppZ_Wf : rexpr_wfT roppZ. Proof. prove_rexpr_wfT. Qed.
+Local Obligation Tactic := rexpr_correct_and_bounded_obligation_tac.
+Program Definition roppZ_correct_and_bounded_tight
+  : rexpr_correct_and_boundedT roppZ roppW ExprUnOp_bounds ropp_output_bounds
+  := rexpr_correct_and_bounded roppZ roppW ExprUnOp_bounds ropp_output_bounds roppZ_Wf.
 
 Local Open Scope string_scope.
-Compute ("Opp", compute_bounds_for_display roppW ExprUnOp_bounds).
-Compute ("Opp overflows? ", sanity_compute roppW ExprUnOp_bounds).
-Compute ("Opp overflows (error if it does)? ", sanity_check roppW ExprUnOp_bounds).
+Compute ("Opp", compute_bounds_for_display roppW_pkg).
+(* We use [compute] rather than [vm_compute] so as to not eta-expand functions, so we get pretty display *)
+Eval compute in ("Opp overflows? ", sanity_compute roppW_pkg).
+Compute ("Opp overflows (error if it does)? ", sanity_check roppW_pkg).
