src/Specific/GF25519Reflective/Reified/Pack.v
@@ -1,17 +1,21 @@
-Require Import Crypto.Specific.GF25519Reflective.CommonUnOpFEToWire.
+Require Import Crypto.Specific.GF25519Reflective.Common.
 
 Definition rpackZ_sig : rexpr_unop_FEToWire_sig pack. Proof. reify_sig. Defined.
-Definition rpackW := Eval vm_compute in rword_of_Z rpackZ_sig.
-Lemma rpackW_correct_and_bounded_gen : correct_and_bounded_genT rpackW rpackZ_sig.
-Proof. rexpr_correct. Qed.
-Definition rpack_output_bounds := Eval vm_compute in compute_bounds rpackW ExprUnOpFEToWire_bounds.
-Local Obligation Tactic := intros; vm_compute; constructor.
-Program Definition rpackW_correct_and_bounded
-  := ExprUnOpFEToWire_correct_and_bounded
-       rpackW pack rpackZ_sig rpackW_correct_and_bounded_gen
-       _ _.
+Definition rpackZ : Expr _ := Eval vm_compute in proj1_sig rpackZ_sig.
+Definition rpackW_pkgo := Eval vm_compute in rexpr_select_word_sizes_option rpackZ ExprUnOpFEToWire_bounds.
+Definition rpackW_pkg := Eval vm_compute in rexpr_select_word_sizes_postprocess1 rpackW_pkgo.
+Definition rpackT := get_output_type rpackW_pkg.
+Definition rpackW' : Expr _ := Eval vm_compute in get_output_expr rpackW_pkg.
+Definition rpackW : Expr rpackT := Eval cbv [rpackW'] in rexpr_select_word_sizes_postprocess2 rpackW'.
+Definition rpack_output_bounds := Eval vm_compute in get_bounds rpackW_pkg.
+Definition rpackZ_Wf : rexpr_wfT rpackZ. Proof. prove_rexpr_wfT. Qed.
+Local Obligation Tactic := rexpr_correct_and_bounded_obligation_tac.
+Program Definition rpackZ_correct_and_bounded_tight
+  : rexpr_correct_and_boundedT rpackZ rpackW ExprUnOpFEToWire_bounds rpack_output_bounds
+  := rexpr_correct_and_bounded rpackZ rpackW ExprUnOpFEToWire_bounds rpack_output_bounds rpackZ_Wf.
 
 Local Open Scope string_scope.
-Compute ("Pack", compute_bounds_for_display rpackW ExprUnOpFEToWire_bounds).
-Compute ("Pack overflows? ", sanity_compute rpackW ExprUnOpFEToWire_bounds).
-Compute ("Pack overflows (error if it does)? ", sanity_check rpackW ExprUnOpFEToWire_bounds).
+Compute ("Pack", compute_bounds_for_display rpackW_pkg).
+(* We use [compute] rather than [vm_compute] so as to not eta-expand functions, so we get pretty display *)
+Eval compute in ("Pack overflows? ", sanity_compute rpackW_pkg).
+Compute ("Pack overflows (error if it does)? ", sanity_check rpackW_pkg).
