src/SpecificGen/GF41417_32Reflective/Reified/CarryAdd.v
@@ -1,17 +1,16 @@
-Require Import Crypto.SpecificGen.GF41417_32Reflective.CommonBinOp.
+Require Import Crypto.SpecificGen.GF41417_32Reflective.Common.
 
 Definition rcarry_addZ_sig : rexpr_binop_sig carry_add. Proof. reify_sig. Defined.
-Definition rcarry_addW := Eval vm_compute in rword_of_Z rcarry_addZ_sig.
-Lemma rcarry_addW_correct_and_bounded_gen : correct_and_bounded_genT rcarry_addW rcarry_addZ_sig.
-Proof. rexpr_correct. Qed.
-Definition rcarry_add_output_bounds := Eval vm_compute in compute_bounds rcarry_addW ExprBinOp_bounds.
+Definition rcarry_addZ : Syntax.Expr _ _ _ := Eval vm_compute in proj1_sig rcarry_addZ_sig.
+Definition rcarry_addW : Syntax.Expr _ _ _ := Eval vm_compute in rexpr_select_word_sizes rcarry_addZ ExprBinOp_bounds.
+Definition rcarry_addZ_Wf : rexpr_wfT rcarry_addZ. Proof. prove_rexpr_wfT. Qed.
+Definition rcarry_add_output_bounds
+  := Eval vm_compute in compute_bounds rcarry_addZ ExprBinOp_bounds.
 Local Obligation Tactic := intros; vm_compute; constructor.
-Program Definition rcarry_addW_correct_and_bounded
-  := ExprBinOp_correct_and_bounded
-       rcarry_addW carry_add rcarry_addZ_sig rcarry_addW_correct_and_bounded_gen
-       _ _.
+Program Definition rcarry_addZ_correct_and_bounded
+  := rexpr_correct_and_bounded rcarry_addZ rcarry_addZ_Wf ExprBinOp_bounds.
 
 Local Open Scope string_scope.
-Compute ("Carry_Add", compute_bounds_for_display rcarry_addW ExprBinOp_bounds).
-Compute ("Carry_Add overflows? ", sanity_compute rcarry_addW ExprBinOp_bounds).
-Compute ("Carry_Add overflows (error if it does)? ", sanity_check rcarry_addW ExprBinOp_bounds).
+Compute ("Carry_Add", compute_bounds_for_display rcarry_addZ ExprBinOp_bounds).
+Compute ("Carry_Add overflows? ", sanity_compute rcarry_addZ ExprBinOp_bounds).
+Compute ("Carry_Add overflows (error if it does)? ", sanity_check rcarry_addZ ExprBinOp_bounds).
